\documentclass[11pt]{report}
\usepackage{amsmath}
\usepackage{mathtools}
\usepackage{amsfonts} 


\title{Computational Finance\\ Exercise Set I}
\author{Georgios Smyridis}


\begin{document}
\maketitle


\section*{Exercise 1}
First, I am going to prove the property $\mathbb{E}[(X-\mathbb{E}[X])^2]=\mathbb{E}[X^2]-\mathbb{E}[X]^2$.
\begin{align}
	\mathbb{E}[(X-\mathbb{E}[X])^2]&=\mathbb{E}\big[X^2-2\mathbb{E}[X]X+\mathbb{E}[X]^2\big]\nonumber\\
	&=\mathbb{E}[X^2]+\mathbb{E}\big[-2E[X]X\big]+\mathbb{E}\big[\mathbb{E}[X]^2\big]\nonumber\\
	&=\mathbb{E}[X^2]-2\mathbb{E}[X]\mathbb{E}[X]+\mathbb{E}[X]^2\nonumber\\
	&=\mathbb{E}[X^2]-\mathbb{E}[X]^2.\nonumber
\end{align}
In the second line, we used the property of expectation values $\mathbb{E}[X+Y]=\mathbb{E}[X]+\mathbb{E}[Y]$. In the third line, we used the property $\mathbb{E}[\alpha X]=\alpha\mathbb{E}[X]$.

Now, with this property, it is easy to show that $\mathbb{V}ar[\alpha X]=\alpha\mathbb{V}ar[X]$. By definition, $\mathbb{V}ar[X]=\mathbb{E}[(X-\mathbb{E}[X])^2]=\mathbb{E}[X^2]-\mathbb{E}[X]^2$. Therefore,
\begin{align}
	\mathbb{V}ar[\alpha X]&=\mathbb{E}[(\alpha X)^2]-\mathbb{E}[\alpha X]^2\nonumber\\
	&=\mathbb{E}[\alpha^2 X^2]-(\alpha\mathbb{E}[X])^2\nonumber\\
	&=\alpha^2\mathbb{E}[X^2]-\alpha^2\mathbb{E}[X]^2\nonumber\\
	&=\alpha^2(\mathbb{E}[X^2]-\mathbb{E}[X]^2)\nonumber\\
	&=\alpha^2\mathbb{V}ar[X],\nonumber
\end{align}
where, again, we have used the two properties of expectation values mentioned above.


\section*{Exercise 6}

The goal of this exercise is to prove that the standard distribution function $F_{\mathcal{N}(0,1)}(x)$, define by
\begin{align}
	F_{\mathcal{N}(0,1)}(x)=\frac1{\sqrt{2\pi}}\int_{-\infty}^x ds\ \exp\bigg(\frac{-s^2}{2}\bigg),
\end{align}
can be calculated with the so-called error function
\begin{align}
	\text{erf}(x)=\frac2{\sqrt{\pi}}\int_0^x ds\ \exp\big(-s^2),
\end{align}
with the help of the relationship
\begin{align}
	F_{\mathcal{N}(0,1)}(x)=\frac12\bigg[1+\text{erf}\bigg(\frac{x}{\sqrt{2}}\bigg)\bigg]
\end{align}
To demonstrate this, one can start from the very definition of the standard distribution function
\begin{align}
	F_{\mathcal{N}(0,1)}&=\frac1{\sqrt{2\pi}}\int_{-\infty}^x ds\ \exp\bigg(\frac{-s^2}2\bigg)\nonumber\\
	&=\frac1{\sqrt{2\pi}}\bigg[\int_{-\infty}^0ds\ \exp\bigg(\frac{-s^2}2\bigg)+\int_0^x ds\ \exp\bigg(\frac{-s^2}2\bigg)\bigg]\nonumber\\
	&=\frac1{\sqrt{2\pi}}\bigg[\sqrt{\frac{\pi}2}+\text{erf}\bigg(\frac{x}{\sqrt{2}}\bigg)\bigg]\nonumber\\
	&=\frac12\bigg[1+\text{erf}\bigg(\frac{x}{\sqrt{2}}\bigg)\bigg]
\end{align}


\end{document}
